src/named/SimpleUnit.v
@@ -11,46 +11,43 @@ Import Core.Notations.
 
 Require Coq.derive.Derive.
 
-Definition unit_lang :=
-  [
+Definition unit_lang_def : lang :=
+  [[l
+  [:|
+     -----------------------------------------------
+      #"unit" : #"ty"
+  ];
+  [:| "G" : #"env"
+      -----------------------------------------------
+      #"tt" : #"val" %"G" #"unit"
+    ];
   [:> "G" : #"env",
       "G'" : #"env",
       "g" : #"sub" %"G'" %"G"
       ----------------------------------------------- ("tt_subst")
       #"val_subst" %"g" #"tt" = #"tt"
       : #"val" %"G'" #"unit"
-  ];
-  (*TODO: design choice: I could add an alalogous expression,
-    and I might autogenerate one at some point, 
-    but it would be equal to ret tt, so I won't for now
-   *)
-  [:| "G" : #"env"
-      -----------------------------------------------
-      #"tt" : #"val" %"G" #"unit"
-    ];
-  [:|
-     -----------------------------------------------
-      #"unit" : #"ty"
-  ]]%arule.
+  ]
+  ]].
 
 
-Derive unit_elab
-       SuchThat (Pre.elab_lang subst_elab unit_lang unit_elab)
+Derive unit_lang
+       SuchThat (Pre.elab_lang value_subst unit_lang_def unit_lang)
        As unit_wf.
 Proof. auto_elab. Qed.
 #[export] Hint Resolve unit_wf : elab_pfs.
 
-Definition unit_eta :=
-  [[:> "G" : #"env",
+Definition unit_eta_def :lang :=
+  [[l [:> "G" : #"env",
        "v" : #"val" %"G" #"unit"
       ----------------------------------------------- ("unit eta")
       %"v" = #"tt"
       : #"val" %"G" #"unit"
-  ]]%arule.
+  ] ]].
 
 
-Derive unit_eta_elab
-       SuchThat (Pre.elab_lang (unit_elab ++ subst_elab) unit_eta unit_eta_elab)
+Derive unit_eta
+       SuchThat (Pre.elab_lang (unit_lang ++ value_subst) unit_eta_def unit_eta)
        As unit_eta_wf.
 Proof. auto_elab. Qed.
 #[export] Hint Resolve unit_eta_wf : elab_pfs.
